\documentclass[11pt]{article}
\usepackage{amsmath}
\usepackage{url}
\begin{document}

\title{\textbf{Arithmetic and Geometric Progression}}
\maketitle
{\Large \textbf{\underline{Introduction}}}
\\
\textbf{Arithmetic progression} refers to a sequence of numbers in which the difference in consecutive terms is constant \textbf{\cite{Aparticle}}.For instance 1,4,7,10,13 is arithmetic progression with difference between consecutive terms is constant ( 3 in this case).\\
If first term of this sequence is $a_1$ and common difference is $d$ , then the $nth$ term of the sequence ($a_n$) is given by: 
$$ a_n = a_1 + (n-1)d $$
\\
Sum of arithmetic progression for n terms is given by:
$$S_n = \frac{n}{2}(a_1 + a_n) $$ 
\begin{center}
\textbf{OR}
\end{center}
$$S_n = \frac{n}{2}(2a_1 + (n-1)d) $$
{\Large \textbf{\underline{Derivation}}}
\begin{align*}
S_n &= a_1 + (a_1 + d) + (a_1 + 2d) + ... + (a_1 + (n-2)d) + (a_1 + (n-1)d)\\
 &= na_1 + d(1 + 2 + 3 + .... + (n-2) + (n-1) ) \\
 &= na_1 + d\frac{n(n-1)}{2}\\
 &= \frac{n}{2}(2a_1 + (n-1)d) \\
a_n &= a_1 + (n-1)d\\
S_n &= \frac{n}{2}(a_1 + a_n) \\
\end{align*}
\\
{\Large \textbf{Geometric Progression}} refers to a sequence of numbers in which each consecutive number is obtained by multiplying a fixed,non zero number to the previous number \textbf{\cite{Gparticle}}. The constant term is called the common ratio. For instance 1,2,4,8,16,.. is a geometric progression with common ratio 2.The general form of a sequence is \\
$$ a, ar^2 , ar^3 , ar^4 , ar^5 .... $$
with common ratio $r$ 
If first term of this sequence is $a_1$ and common ratio is $r$ , then the $nth$ term of the sequence ($a_n$) is given by: 
$$ a_n = a_1r^n $$
Sum of geometric progression for n terms is given by:
$$S_n=a_1 (\frac{1-r^n}{1-r})$$
{\Large \textbf{\underline{Derivation}}}
$$ \sum\limits_{i=1}^n ar^{k-1} = ar^0 + ar^1 + ar^2+ ..... + ar^{n-1} $$
Now multiplying the above term by $r$ and subtracting it from the above
 \begin{align*} 
(1-r)\sum\limits_{i=1}^n ar^{k-1} &= ar^0 + ar^1 + ar^2+ ............. + ar^{n-1}\\
 & \hspace{10mm}-ar^1 -ar^2..................-ar^{n-1} - ar^n\\
 &= ar^0 - ar^n\\
\sum\limits_{i=1}^n ar^{k-1} &= a\frac{1 - r^n}{1-r}\\
S_n &= a\frac{1 - r^n}{1-r}
\end{align*}
\bibliography{cite}
\bibliographystyle{plain}



\end{document}